# Derivatives of Functions

### 1. \( y(x) = -3x + 3 \)
The derivative is:
$$y'(x) = -3$$

---

### 2. \( y(x) = \pi x + \sin(1) \)
The derivative is:
$$y'(x) = \pi$$
(Note: \(\sin(1)\) is a constant, so its derivative is 0.)

---

### 3. \( y(x) = 4 + \sin(2) \)
The derivative is:
$$y'(x) = 0$$
(Both 4 and \(\sin(2)\) are constants.)

---

### 4. \( y(x) = 2x^3 - 3x^2 + 8x - 9 \)
Differentiate term by term:
$$y'(x) = 6x^2 - 6x + 8$$

---

### 5. \( y(x) = 6x^{1/3} \)
Using the power rule \( \frac{d}{dx} x^n = n x^{n-1} \):
$$y'(x) = 6 \cdot \frac{1}{3} x^{-2/3} = \frac{2}{x^{2/3}}$$

---

### 6. \( y(x) = \sqrt{x} \)
Rewrite \( \sqrt{x} = x^{1/2} \), then use the power rule:
$$y'(x) = \frac{1}{2} x^{-1/2} = \frac{1}{2\sqrt{x}}$$

---

### 7. \( y(x) = \cos(x) + \sin(x) \)
The derivative is:
$$y'(x) = -\sin(x) + \cos(x)$$

---

### 8. \( y(x) = 2\sin(x)\cos(x) \)
This is a product, so use the product rule or simplify using the double-angle identity \( \sin(2x) = 2\sin(x)\cos(x) \):
$$y'(x) = \cos(2x)$$

---

### 9. \( y(x) = x\sin(x) \)
Use the product rule \( \frac{d}{dx}[uv] = u'v + uv' \):
$$y'(x) = 1\cdot\sin(x) + x\cos(x) = \sin(x) + x\cos(x)$$

---

### 10. \( y(x) = (x + 1)(x + 1) \)
Simplify as \( y(x) = (x + 1)^2 \), then use the chain rule:
$$y'(x) = 2(x + 1)$$

---

### 11. \( y(x) = -\frac{x}{x + 1} \)
Use the quotient rule:
$$y'(x) = \frac{(-1)(x+1) - (-x)(1)}{(x+1)^2} = \frac{-x - 1 + x}{(x+1)^2} = \frac{-1}{(x+1)^2}$$

---

### 12. \( y(x) = (x + 1)e^x \)
Use the product rule:
$$y'(x) = (1)e^x + (x+1)e^x = e^x + xe^x = (x+1)e^x$$

---

### 13. \( y(x) = \sin(x^2) \)
Use the chain rule:
$$y'(x) = \cos(x^2) \cdot 2x = 2x\cos(x^2)$$

---

### 14. \( y(x) = e^{(-2x)} \)
Use the chain rule:
$$y'(x) = e^{-2x} \cdot (-2) = -2e^{-2x}$$

---

### 15. \( y(x) = \frac{1}{\sin(x+1)} \)
Rewrite as \( y(x) = (\sin(x+1))^{-1} \), then use the chain rule:
$$y'(x) = -(\sin(x+1))^{-2} \cdot \cos(x+1) = -\frac{\cos(x+1)}{\sin^2(x+1)}$$

---

### 16. \( y(x) = \sqrt{2x + 1} \)
Rewrite as \( y(x) = (2x+1)^{1/2} \), then use the chain rule:
$$y'(x) = \frac{1}{2}(2x+1)^{-1/2} \cdot 2 = \frac{1}{\sqrt{2x+1}}$$

---
