
# Conic Curves

## Q1
Given:  
$$
A = (1, 2), \quad R = 3
$$

The general equation of a circle is:  
$$
(x - h)^2 + (y - k)^2 = R^2
$$

Substituting:  
$$
h = 1, \quad k = 2, \quad R = 3
$$

The equation becomes:  
$$
(x - 1)^2 + (y - 2)^2 = 3^2
$$  
$$
(x - 1)^2 + (y - 2)^2 = 9
$$

---

## Q2
Given:  
$$
x_1 = 2, \quad x_2 = 4, \quad \text{Point } (3, 1)
$$

The general equation of a parabola is:  
$$
y = a (x - x_1)(x - x_2)
$$

Substituting:  
$$
1 = a (3 - 2)(3 - 4)
$$  
$$
1 = a (1)(-1)
$$  
$$
a = -1
$$

Thus, the equation becomes:  
$$
y = -1 (x - 2)(x - 4)
$$  
$$
y = - (x^2 - 6x + 8)
$$  
$$
y = -x^2 + 6x - 8
$$